lots of work on alpha-congrunce in lambdas
Ignore-this: fbbec9dac4cb328ff4e0b25df646e0c7

darcs-hash:20140225035601-f399b-8539c3aa0b4d34be642abfb614ced7c27e4f9f69

st_lam.v
@@ -30,6 +30,10 @@ Inductive ty :=
 Delimit Scope ty_scope with ty.
 
 Notation "x ⇒ y" := (ty_arrow x y) : ty_scope.
+Bind Scope ty_scope with ty.
+
+Delimit Scope lam_scope with lam.
+Open Scope lam_scope.
 
 Definition env := list (atom * ty).
 
@@ -69,16 +73,16 @@ Inductive term (Γ:env) : ty -> Type :=
   | tbool : forall n:bool,
                 term Γ ty_bool
   | tapp : forall σ₁ σ₂,
-                term Γ (σ₁ ⇒ σ₂)%ty ->
+                term Γ (σ₁ ⇒ σ₂) ->
                 term Γ σ₁ ->
                 term Γ σ₂
   | tlam : forall x σ₁ σ₂,
                 term ((x,σ₁)::Γ) σ₂ ->
-                term Γ (σ₁ ⇒ σ₂)%ty.
-Arguments term Γ ty%ty.
+                term Γ (σ₁ ⇒ σ₂).
 
-Local Open Scope ty.
-
+Arguments tapp [_ _ _] _ _.
+Notation "x • y" := (tapp x y) 
+  (at level 52, left associativity, format "x • y") : lam_scope.
 
 Definition concat A := fold_right (@app A) nil.
 
@@ -111,30 +115,37 @@ Fixpoint term_papp (p:perm) Γ τ (m:term Γ τ) : term (env_papp p Γ) τ :=
   match m with
   | tvar x σ H => tvar _ (p x) σ (inenv_papp Γ x σ p H)
   | tbool b => tbool _ b
-  | tapp σ₁ σ₂ m1 m2 => tapp _ σ₁ σ₂ (term_papp p _ _ m1) (term_papp p _ _ m2)
+  | tapp σ₁ σ₂ m1 m2 => tapp (term_papp p _ _ m1) (term_papp p _ _ m2)
   | tlam x σ₁ σ₂ m' => tlam _ (p x) σ₁ σ₂ (term_papp p _ _ m')
   end.
 
-Inductive alpha_eq : forall Γ Γ' (ρ₁ ρ₂:perm) (τ:ty),
-  term Γ τ -> term Γ' τ -> Prop :=
+Inductive var_cong : env -> env -> atom -> atom -> Prop :=
+ | vcong_here : forall Γ₁ Γ₂ x₁ x₂ y₁ y₂ τ, 
+                   x₁ = y₁ -> x₂ = y₂ ->
+                   var_cong ((x₁,τ)::Γ₁) ((x₂,τ)::Γ₂) y₁ y₂
+ | vcong_there : forall Γ₁ Γ₂ x₁ x₂ y₁ y₂ τ,
+                   x₁ <> y₁ -> x₂ <> y₂ ->
+                   var_cong Γ₁ Γ₂ y₁ y₂ ->
+                   var_cong ((x₁,τ)::Γ₁) ((x₂,τ)::Γ₂) y₁ y₂.
 
-  | aeq_var : forall Γ Γ' (ρ₁ ρ₂:perm) τ x₁ x₂ H₁ H₂,
-                  ρ₁ x₁ = ρ₂ x₂ ->
-                  alpha_eq Γ Γ' ρ₁ ρ₂ τ (tvar Γ x₁ τ H₁) (tvar Γ' x₂ τ H₂)
+Inductive alpha_cong : forall Γ Γ' (τ:ty), term Γ τ -> term Γ' τ -> Prop :=
 
-  | aeq_bool : forall Γ Γ' ρ₁ ρ₂ b,
-                  alpha_eq Γ Γ' ρ₁ ρ₂ ty_bool
-                    (tbool Γ b) (tbool Γ' b)
+  | acong_var : forall Γ Γ' τ x₁ x₂ H₁ H₂,
+                  var_cong Γ Γ' x₁ x₂ ->
+                  alpha_cong Γ Γ' τ (tvar Γ x₁ τ H₁) (tvar Γ' x₂ τ H₂)
 
-  | aeq_app : forall Γ Γ' ρ₁ ρ₂ σ₁ σ₂ m₁ m₂ n₁ n₂,
-                  alpha_eq Γ Γ' ρ₁ ρ₂ (σ₁ ⇒ σ₂) m₁ n₁ ->
-                  alpha_eq Γ Γ' ρ₁ ρ₂ σ₁ m₂ n₂ ->
-                  alpha_eq Γ Γ' ρ₁ ρ₂ σ₂ (tapp Γ σ₁ σ₂ m₁ m₂) (tapp Γ' σ₁ σ₂ n₁ n₂)
+  | acong_bool : forall Γ Γ' b,
+                  alpha_cong Γ Γ' ty_bool (tbool Γ b) (tbool Γ' b)
 
-  | aeq_lam : forall (Γ Γ':env) (ρ₁ ρ₂:perm) (x₁ x₂ x:atom) σ₁ σ₂ m₁ m₂,
-                  x♯x₁ -> x♯x₂ -> x♯ρ₁ -> x♯ρ₂ -> x♯Γ -> x♯Γ' ->
-                  alpha_eq ((x₁,σ₁)::Γ) ((x₂,σ₁)::Γ') (ρ₁ ∘ x ⇋ x₁) (ρ₂ ∘ x ⇋ x₂) σ₂ m₁ m₂ ->
-                  alpha_eq Γ Γ' ρ₁ ρ₂ (σ₁ ⇒ σ₂) (tlam Γ x₁ σ₁ σ₂ m₁) (tlam Γ' x₂ σ₁ σ₂ m₂).
+  | acong_app : forall Γ Γ' σ₁ σ₂ m₁ m₂ n₁ n₂,
+                  alpha_cong Γ Γ' (σ₁ ⇒ σ₂) m₁ n₁ ->
+                  alpha_cong Γ Γ' σ₁ m₂ n₂ ->
+                  alpha_cong Γ Γ' σ₂ (m₁ • m₂) (n₁ • n₂)
+
+  | acong_lam : forall (Γ Γ':env) (x₁ x₂:atom) σ₁ σ₂ m₁ m₂,
+                  alpha_cong ((x₁,σ₁)::Γ) ((x₂,σ₁)::Γ') σ₂ m₁ m₂ ->
+                  alpha_cong Γ Γ' (σ₁ ⇒ σ₂) (tlam Γ x₁ σ₁ σ₂ m₁) (tlam Γ' x₂ σ₁ σ₂ m₂).
+
 
 Fixpoint raw (Γ:env) (τ:ty) (m:term Γ τ) : rawterm :=
   match m with
@@ -165,7 +176,7 @@ Fixpoint term_wk (Γ₁ Γ₂:env) (σ:ty)
   | tvar x σ IN => tvar Γ₂ x σ (H x σ IN)
   | tbool b => tbool Γ₂ b
   | tapp σ₁ σ₂ m₁ m₂ =>
-        tapp Γ₂ σ₁ σ₂ (term_wk Γ₁ Γ₂ (σ₁ ⇒ σ₂) m₁ H) (term_wk Γ₁ Γ₂ σ₁ m₂ H)
+        @tapp Γ₂ σ₁ σ₂ (term_wk Γ₁ Γ₂ (σ₁ ⇒ σ₂) m₁ H) (term_wk Γ₁ Γ₂ σ₁ m₂ H)
   | tlam x σ₁ σ₂ m' =>
         tlam Γ₂ x σ₁ σ₂ 
             (term_wk ((x,σ₁)::Γ₁) ((x,σ₁)::Γ₂) σ₂ m'
@@ -255,15 +266,15 @@ Proof.
 Defined.
 
 Fixpoint term_subst
-  (Γ Γ':env) (τ₁:ty)
+  (Γ Γ':env) (τ:ty)
   (VAR:varmap Γ Γ')
-  (m:term Γ τ₁) : term Γ' τ₁ :=
+  (m:term Γ τ) : term Γ' τ :=
 
   match m with
   | tvar x σ IN => VAR x σ IN
   | tbool b => tbool Γ' b
   | tapp σ₁ σ₂ m₁ m₂ =>
-      tapp Γ' σ₁ σ₂
+      @tapp Γ' σ₁ σ₂
           (term_subst Γ Γ' (σ₁ ⇒ σ₂) VAR m₁)
           (term_subst Γ Γ' σ₁ VAR m₂)
   | tlam x σ₁ σ₂ m' =>
@@ -283,38 +294,365 @@ Program Definition term1 :=
   tlam (("x",ty_bool)::nil) "y" ty_bool ty_bool
     (tvar (("y",ty_bool)::("x",ty_bool)::nil) "x" ty_bool (Logic.refl_equal _)).
 
+Program Definition term1' :=
+  tlam (("x",ty_bool)::nil) "x" ty_bool ty_bool
+    (tvar (("x",ty_bool)::("x",ty_bool)::nil) "x" ty_bool (Logic.refl_equal _)).
+
 Program Definition term2 :=
   tbool nil false.
 
-Definition term3' := subst nil _ _ "x" term1 term2.
+Definition term3 := subst nil _ _ "x" term1 term2.
+Definition term3' := subst nil _ _ "x" term1' term2.
 
-Program Definition term3 :=
-  subst nil (ty_bool ⇒ ty_bool) ty_bool "x" term1 term2.
+Program Definition term1'' :=
+  tlam nil "x" ty_bool ty_bool
+    (tvar (("x",ty_bool)::nil) "x" ty_bool (Logic.refl_equal _)).
+
+Definition term4 := subst nil _ _ "x" term1 (term1'' • tbool _ true).
+Definition term4' := subst nil _ _ "x" term1' (term1'' • tbool _ true).
+
+Program Definition term5 :=
+  tlam (("y",ty_bool ⇒ ty_bool)%ty::("x",ty_bool)%ty::nil) "x" ty_bool _
+    (tvar (("x",ty_bool)::("y",ty_bool ⇒ ty_bool)%ty::("x",ty_bool)%ty::nil) 
+       "y" (ty_bool ⇒ ty_bool) (Logic.refl_equal _)).
+
+Definition term6 := subst (("x",ty_bool)%ty::nil) _ _ "y" term5 term1.
+Definition term6' := subst (("x",ty_bool)%ty::nil) _ _ "y" term5 term1'.
 
 Eval vm_compute in (raw _ _ term1).
+Eval vm_compute in (raw _ _ term1').
 Eval vm_compute in (raw _ _ term2).
 Eval vm_compute in (raw _ _ term3).
 Eval vm_compute in (raw _ _ term3').
+Eval vm_compute in (raw _ _ term4).
+Eval vm_compute in (raw _ _ term4').
+Eval vm_compute in (raw _ _ term5).
+Eval vm_compute in (raw _ _ term6).
+Eval vm_compute in (raw _ _ term6').
 
+
+(**  Syntactic types have decicable equality, which
+     implies injectivity for dependent pairs with
+     (syntactic) types as the type being depended upon.
+  *)
+Lemma inj_pair2_ty : forall (F:ty -> Type) τ x y,
+  existT F τ x = existT F τ y -> x = y.
+Proof.
+  intros.
+  apply Eqdep_dec.inj_pair2_eq_dec in H. auto.
+  decide equality.
+Qed.
+
+Lemma env_dec : forall a b:env, {a=b}+{a<>b}.
+Proof.
+  decide equality.
+  decide equality.
+  decide equality.
+  apply string_dec.
+Qed.
+
+Ltac inj_ty :=
+  repeat match goal with
+           [ H : existT _ _ _ = existT _ _ _ |- _ ] =>
+             apply inj_pair2_ty in H ||
+             apply (Eqdep_dec.inj_pair2_eq_dec _ string_dec) in H ||
+             apply (Eqdep_dec.inj_pair2_eq_dec _ env_dec) in H
+           end.
+
+Ltac inv H :=
+  inversion H; subst; inj_ty; repeat subst.
+
+Section varmap_compose.
+  Variables Γ₁ Γ₂ Γ₃:env.
+  Variable g:varmap Γ₂ Γ₃.
+  Variable f:varmap Γ₁ Γ₂.  
+
+  Program Definition varmap_compose : varmap Γ₁ Γ₃ :=
+    fun a τ (IN:inenv Γ₁ a τ) => term_subst Γ₂ Γ₃ τ g (f a τ IN).
+End varmap_compose.
+
+Lemma var_cong_refl Γ x τ:
+  inenv Γ x τ ->
+  var_cong Γ Γ x x.
+Proof.
+  induction Γ; intro H.
+  inv H.
+  hnf in H. simpl in H.
+  destruct a.
+  destruct (string_dec x c). inv H.
+  apply vcong_here; auto.
+  apply vcong_there; auto.
+Qed.
+
+Lemma var_cong_trans Γ₁ Γ₂ x y z :
+  var_cong Γ₁ Γ₂ x y ->
+  forall Γ₃,
+  var_cong Γ₂ Γ₃ y z ->
+  var_cong Γ₁ Γ₃ x z.
+Proof.
+  intro H; induction H; intros.
+  subst. inv H1.
+  apply vcong_here; auto.
+  elim H3; auto.
+  inv H2.
+  elim H0. auto.
+  apply vcong_there; auto.
+Qed.
+
+Lemma alpha_eq_refl Γ σ (m:term Γ σ) :
+  alpha_cong Γ Γ σ m m.
+Proof.
+  induction m.
+  apply acong_var.
+  eapply var_cong_refl; eauto.
+  apply acong_bool.
+  apply acong_app; auto.
+  apply acong_lam; auto.
+Qed.
+
+Lemma alpha_eq_trans Γ₁ τ (m:term Γ₁ τ) : 
+  forall Γ₂ Γ₃ (n:term Γ₂ τ) (o:term Γ₃ τ),
+  alpha_cong Γ₁ Γ₂ τ m n ->
+  alpha_cong Γ₂ Γ₃ τ n o ->
+  alpha_cong Γ₁ Γ₃ τ m o.
+Proof.
+  induction m; intros; inv H; inv H0.
+  apply acong_var.
+  eapply var_cong_trans; eauto.
+  apply acong_bool.
+  apply acong_app; eauto.
+  apply acong_lam; eauto.
+Qed.
+
+Lemma alpha_cong_wk : forall (Γm Γn Γm' Γn':env) τ m n H₁ H₂,
+  (forall a b, var_cong Γm Γn a b -> var_cong Γm' Γn' a b) ->
+  alpha_cong Γm Γn τ m n ->
+  alpha_cong _ _ τ (term_wk Γm Γm' τ m H₁)
+                   (term_wk Γn Γn' τ n H₂).
+Proof.
+  intros. revert Γm' Γn' H₁ H₂ H.
+  induction H0; simpl; intros.
+  apply acong_var. apply H0. auto.
+  apply acong_bool.
+  apply acong_app; auto.
+  apply acong_lam. apply IHalpha_cong.
+  intros. inv H1.
+  apply vcong_here; auto.
+  apply vcong_there; auto.
+Qed.
+
+Lemma term_subst_cong : forall Γ τ (m:term Γ τ) Γ₁ Γ₂ 
+  (VAR1 : varmap Γ Γ₁) (VAR2 : varmap Γ Γ₂),
+  
+  (forall a σ IN, alpha_cong Γ₁ Γ₂ σ (VAR1 a σ IN) (VAR2 a σ IN)) ->
+
+  alpha_cong Γ₁ Γ₂ τ
+    (term_subst Γ Γ₁ τ VAR1 m)
+    (term_subst Γ Γ₂ τ VAR2 m).
+Proof.
+  intros until m; induction m; simpl; intros; auto.
+  apply acong_bool.
+  apply acong_app; auto.
+  apply acong_lam; auto.
+  apply IHm. intros.
+  unfold shift_vars', shift_vars, extend_map, weaken_map.
+  hnf in IN. simpl in IN.
+  revert IN.
+  destruct (string_dec a x); simpl; intros.
+  subst a. inv IN.
+  replace IN with (Logic.eq_refl (Some σ)). simpl.
+  unfold eq_rect_r. simpl.
+  unfold newestvar. simpl.
+  apply acong_var.
+  apply vcong_here; auto.
+  apply Eqdep_dec.UIP_dec. decide equality. decide equality.
+  apply alpha_cong_wk; auto.
+  intros.
+  apply vcong_there; auto.
+admit.
+admit.
+Qed.
+
+Lemma term_wk_ident : forall Γ σ m H,
+  term_wk Γ Γ σ m H = m.
+Proof.
+  intros until m; induction m; simpl; intros; auto.
+  f_equal.
+  apply Eqdep_dec.UIP_dec. decide equality. decide equality.
+  f_equal; auto.
+  f_equal; auto.
+Qed.  
+
+Lemma term_wk_compose : forall Γ₁ σ m Γ₂ Γ₃ H1 H2 H3,
+  term_wk Γ₂ Γ₃ σ (term_wk Γ₁ Γ₂ σ m H1) H2 = term_wk Γ₁ Γ₃ σ m H3.
+Proof.
+  intros until m. induction m; simpl; intros; auto.
+  f_equal.
+  apply Eqdep_dec.UIP_dec. decide equality. decide equality.
+  rewrite (IHm1 Γ₂ Γ₃ H1 H2 H3).
+  rewrite (IHm2 Γ₂ Γ₃ H1 H2 H3).
+  auto.
+  f_equal.
+  apply IHm.
+Qed.
+
+Lemma term_wk_compose' : forall Γ₁ σ m Γ₂ Γ₃ H1 H2,
+  term_wk Γ₂ Γ₃ σ (term_wk Γ₁ Γ₂ σ m H1) H2 = 
+  term_wk Γ₁ Γ₃ σ m (fun x τ H => H2 x τ (H1 x τ H)).
+Proof.
+  intros. eapply term_wk_compose; eauto.
+Qed.
+
+Lemma term_subst_wk_cong : forall Γ τ (m:term Γ τ) Γ₁ Γ₂ Γ₃ Γ₄ 
+  (VAR1 : varmap Γ Γ₁) (VAR2:varmap Γ₃ Γ₄) H₁ H₂,
+
+  (forall a σ Ha1 Ha2 H,
+    alpha_cong _ _ σ (term_wk Γ₁ Γ₂ σ (VAR1 a σ Ha1) H) (VAR2 a σ Ha2)) ->
+
+  alpha_cong _ _ τ
+    (term_wk Γ₁ Γ₂ τ (term_subst Γ Γ₁ τ VAR1 m) H₁)
+    (term_subst Γ₃ Γ₄ τ VAR2 (term_wk Γ Γ₃ τ m H₂)).
+Proof.
+  intros until m. induction m; simpl; intros; auto.
+  apply acong_bool.
+  apply acong_app; auto.
+  apply acong_lam.
+
+  apply IHm; clear IHm.
+  intros. unfold shift_vars'. unfold shift_vars.
+  unfold extend_map. simpl. unfold weaken_map. simpl.
+  unfold newestvar. simpl. unfold newestvar_obligation_1. simpl.
+  generalize Ha1 Ha2. unfold inenv; simpl.
+  destruct (string_dec a x); simpl.
+  subst a. intros.
+  inv Ha0. unfold eq_rect_r.
+  replace Ha0 with (Logic.eq_refl (Some σ)).
+  replace Ha3 with (Logic.eq_refl (Some σ)). simpl.
+  apply acong_var.
+  apply vcong_here; auto.
+  apply Eqdep_dec.UIP_dec. decide equality. decide equality.
+  apply Eqdep_dec.UIP_dec. decide equality. decide equality.
+
+  intros.  
+  rewrite term_wk_compose'.
+  match goal with [ |- alpha_cong _ _ _
+    (term_wk _ _ _ _ ?Q1)
+    (term_wk _ _ _ _ ?Q2) ] =>
+    generalize Q1 Q2; intros
+  end.
+  assert (forall x τ, inenv Γ₂ x τ -> inenv ((fresh[Γ,Γ₂],σ₁)::Γ₂) x τ).
+    intros.
+    hnf. hnf in H1. simpl. simpl in H1.
+    rewrite H1.
+    set (q := fresh [Γ,Γ₂]).
+    simpl in q. fold q.
+    destruct (string_dec x0 q).
+    subst q.
+    elimtype False.
+admit.
+    auto.
+
+  apply alpha_eq_trans with
+    ((fresh [Γ,Γ₂],σ₁)::Γ₂) 
+    (term_wk Γ₂ ((fresh [Γ,Γ₂],σ₁)::Γ₂) σ
+      (term_wk Γ₁ Γ₂ σ (VAR1 a σ Ha0) H₁) H1).
+  rewrite term_wk_compose'.
+  apply alpha_cong_wk.
+admit.
+  apply alpha_eq_refl.
+  apply alpha_cong_wk.
+  intros.
+  apply vcong_there.
+admit.
+admit.
+  auto.
+  apply H.
+Qed.
+
+
+Lemma compose_term_subst : forall Γ₁ τ (m:term Γ₁ τ),
+  forall (Γ₂ Γ₃:env) (g:varmap Γ₂ Γ₃) (f:varmap Γ₁ Γ₂),
+  alpha_cong _ _ _ 
+    (term_subst Γ₁ Γ₃ τ (varmap_compose _ _ _ g f) m)
+    (term_subst Γ₂ Γ₃ τ g (term_subst Γ₁ Γ₂ τ f m)).
+Proof.
+  unfold varmap_compose.
+  do 3 intro. induction m; simpl; intros.
+  apply alpha_eq_refl.
+  apply acong_bool.
+  simpl. apply acong_app.
+  apply IHm1; auto.
+  apply IHm2; auto.
+
+  apply acong_lam.
+  eapply alpha_eq_trans. 2: apply IHm.
+
+  apply term_subst_cong.
+  clear. unfold shift_vars', shift_vars. simpl.
+  intros.
+  simpl.
+  unfold inenv in *. simpl in *.
+  unfold extend_map.
+  destruct (string_dec a x).
+  unfold eq_rect_r. simpl.
+  subst a. inv IN.
+  replace IN with (Logic.eq_refl (Some σ)).
+  simpl.
+  set (q := (fresh_atom (‖Γ‖ ++ ‖Γ₂‖ ++ nil))).
+  simpl in *. fold q.
+  unfold newestvar_obligation_1.
+  destruct (string_dec q q).
+  simpl. unfold newestvar. simpl.
+  apply acong_var.
+  apply vcong_here; auto.
+  elim n; auto.
+  apply Eqdep_dec.UIP_dec. decide equality. decide equality.
+
+  apply term_subst_wk_cong. simpl. intros.
+  set (q1 := fresh [ Γ, Γ₂ ]). 
+  set (q2 := fresh [ Γ₂, Γ₃ ]).
+  unfold inenv in *. simpl in *.
+  revert Ha2.
+  simpl in *. fold q1. fold q2.  
+  destruct (string_dec a0 q1).
+  subst a0.
+  elimtype False.
+  revert Ha1.
+admit.
+  intros.
+  apply alpha_cong_wk.
+  intros. apply vcong_there; auto.
+admit.
+  unfold q2.
+admit.
+  replace Ha2 with Ha1.
+  apply alpha_eq_refl.
+  apply Eqdep_dec.UIP_dec. decide equality. decide equality.
+Qed.  
+
+
+Reserved Notation "m ⇓ z" (at level 82, left associativity).
+Reserved Notation "m ↓" (at level 82, left associativity).
 
 Inductive eval (Γ:env) : forall τ, term Γ τ -> term Γ τ -> Prop :=
   | evar : forall x τ IN,
-               eval Γ τ (tvar Γ x τ IN) (tvar Γ x τ IN)
+               tvar Γ x τ IN ↓
   | ebool : forall b,
-               eval Γ ty_bool (tbool Γ b) (tbool Γ b)
+               tbool Γ b ↓
   | elam : forall x σ₁ σ₂ m,
-               eval Γ (σ₁ ⇒ σ₂) (tlam Γ x σ₁ σ₂ m) (tlam Γ x σ₁ σ₂ m)
+               tlam Γ x σ₁ σ₂ m ↓
   | eapp : forall x σ₁ σ₂ m₁ m₂ n₁ n₂ z,
-               eval Γ (σ₁ ⇒ σ₂) m₁ (tlam Γ x σ₁ σ₂ n₁) ->
-               eval Γ σ₁ m₂ n₂ ->
-               eval Γ σ₂ (subst Γ σ₂ σ₁ x n₁ n₂) z ->
-               eval Γ σ₂ (tapp Γ σ₁ σ₂ m₁ m₂) z.
-
+               m₁ ⇓ (tlam Γ x σ₁ σ₂ n₁) ->
+               m₂ ⇓ n₂ ->
+               subst Γ σ₂ σ₁ x n₁ n₂ ⇓ z ->
+               m₁ • m₂ ⇓ z
+ where "m ⇓ z" := (eval _ _ m z)
+  and "m ↓" := (eval _ _ m m).
 
 Fixpoint tydom (τ:ty) : PLT :=
   match τ with
   | ty_bool => disc finbool
-  | ty_arrow τ₁ τ₂ => PLT.exp (tydom τ₁) (tydom τ₂)
+  | (τ₁ ⇒ τ₂)%ty => tydom τ₁ ⇒ tydom τ₂
   end.
 
 Notation cxt := (finprod.finprod false string string_dec ty tydom).
@@ -329,6 +667,550 @@ Fixpoint denote (Γ:env) (τ:ty) (m:term Γ τ) : dom Γ τ :=
   match m in term _ τ' return dom Γ τ' with
   | tvar x σ IN => castty IN ∘ proj Γ x
   | tbool b => disc_elem b ∘ PLT.terminate false (cxt Γ)
-  | tapp σ₁ σ₂ m₁ m₂ => apply ∘ 〈 denote Γ (σ₁ ⇒ σ₂)%ty m₁, denote Γ σ₁ m₂ 〉
-  | tlam x σ₁ σ₂ m' => Λ(denote ((x,σ₁)::Γ) σ₂ m' ∘ bind Γ x σ₁)
+  | tapp σ₁ σ₂ m₁ m₂ => apply ∘ 〈 〚m₁〛, 〚m₂〛 〉
+  | tlam x σ₁ σ₂ m' => Λ(〚m'〛 ∘ bind Γ x σ₁)
+  end
+ where "〚 m 〛" := (denote _ _ m) : lam_scope.
+
+(* FIXME: move to profinite.v *)
+Lemma plt_terminate_univ : forall (A:PLT) (f:A → 1),
+  f ≈ PLT.terminate false A.
+Proof.
+  intros. split.
+  apply PLT.terminate_le_univ.
+  hnf; simpl; intros.
+  destruct a.
+  destruct u.
+  destruct (PLT.hom_directed false _ _ f c nil); auto.
+  hnf; auto. hnf; intros. apply nil_elem in H0. elim H0.
+  destruct H0. apply erel_image_elem in H1. destruct x. auto.
+Qed.
+
+Lemma alpha_cong_denote (Γ₁ Γ₂:env) τ (m:term Γ₁ τ) (n:term Γ₂ τ) :
+  alpha_cong Γ₁ Γ₂ τ m n -> 
+
+  forall A (h₁:A → cxt Γ₁) (h₂:A → cxt Γ₂),
+
+  (forall a b τ (IN1:inenv Γ₁ a τ) (IN2:inenv Γ₂ b τ),
+    var_cong Γ₁ Γ₂ a b ->
+    castty IN1 ∘ proj Γ₁ a ∘ h₁ ≈ castty IN2 ∘ proj Γ₂ b ∘ h₂) ->
+
+  〚m〛 ∘ h₁ ≈ 〚n〛 ∘ h₂.
+Proof.
+  intro H. induction H.
+  simpl; intros. apply H0. auto.
+  simpl; intros.
+  do 2 rewrite <- (cat_assoc PLT).
+  apply cat_respects; auto.
+  transitivity (PLT.terminate false A).
+  apply plt_terminate_univ.
+  symmetry.
+  apply plt_terminate_univ.
+  simpl; intros.
+  do 2 rewrite <- (cat_assoc PLT).
+  apply cat_respects; auto.
+  do 2 rewrite (PLT.pair_compose_commute false).
+  apply PLT.pair_eq.
+  apply IHalpha_cong1. auto.
+  apply IHalpha_cong2. auto.
+  simpl; intros.
+  do 2 rewrite (PLT.curry_compose_commute false).
+  apply PLT.curry_eq.
+  do 2 rewrite <- (cat_assoc PLT).
+  apply IHalpha_cong.  
+  intros. inv H1.
+  do 2 rewrite <- (cat_assoc PLT).
+  rewrite (cat_assoc PLT _ _ _ _ (proj ((a,σ₁)::Γ) a)).
+  rewrite (finprod.proj_bind false).
+  rewrite <- (cat_assoc PLT).
+  unfold PLT.pair_map.
+  rewrite PLT.pair_commute2.
+  rewrite (cat_ident2 PLT).
+  symmetry.  
+  rewrite (cat_assoc PLT _ _ _ _ (proj ((b,σ₁)::Γ') b)).
+  rewrite (finprod.proj_bind false).
+  rewrite <- (cat_assoc PLT).
+  rewrite PLT.pair_commute2.
+  do 2 rewrite (cat_assoc PLT).
+  apply cat_respects; auto.  
+  etransitivity.
+  apply cast_compose.
+  symmetry.
+  etransitivity.
+  apply cast_compose.
+
+  generalize (Logic.eq_trans (finprod.lookup_eq string string_dec ty Γ a σ₁) IN1).
+  generalize (Logic.eq_trans (finprod.lookup_eq string string_dec ty Γ' b σ₁) IN2).
+  hnf in IN1. simpl in *.
+  destruct (string_dec a a).
+  inv IN1. intros.
+  replace e0 with e1. auto.
+  apply Eqdep_dec.UIP_dec. decide equality. decide equality.
+  elim n; auto.
+
+  do 2 rewrite <- (cat_assoc PLT).
+  rewrite (cat_assoc PLT _ _ _ _ (proj ((x₁,σ₁)::Γ) a)).
+  rewrite (finprod.proj_bind_neq false); auto.
+  instantiate (1:=H9).
+  unfold PLT.pair_map.
+  rewrite <- (cat_assoc PLT).
+  rewrite PLT.pair_commute1.
+  symmetry.
+  rewrite (cat_assoc PLT _ _ _ _ (proj ((x₂,σ₁)::Γ') b)).
+  rewrite (finprod.proj_bind_neq false); auto.
+  instantiate (1:=H10).
+  rewrite <- (cat_assoc PLT).
+  rewrite PLT.pair_commute1.
+  repeat rewrite (cat_assoc PLT).
+  apply cat_respects; auto.
+  rewrite (cast_compose false).  
+  rewrite (cast_compose false).  
+  symmetry. apply H0. auto.
+Qed.  
+
+Lemma alpha_cong_denote_closed τ (m:term nil τ) (n:term nil τ) :
+  alpha_cong nil nil τ m n -> 〚m〛 ≈ 〚n〛.
+Proof.
+  intros.
+  cut (〚m〛∘ id ≈ 〚n〛∘ id ).
+  intro. do 2 rewrite (cat_ident1 PLT) in H0. auto.
+  apply alpha_cong_denote; auto.
+  intros. inv H0.
+Qed.
+
+Definition varmap_denote (Γ Γ':env) (VAR:varmap Γ Γ') : cxt Γ' → cxt Γ.
+Admitted.  
+
+Lemma varmap_extend_bind Γ Γ' 
+ (VAR:varmap Γ Γ') x σ (m:term Γ' σ) :
+
+ varmap_denote _ _ (extend_map Γ Γ' VAR x σ m) ≈
+ bind Γ x σ ∘ 〈 varmap_denote _ _ VAR, 〚m〛〉.
+Admitted.
+
+Lemma varmap_var_id Γ :
+  varmap_denote Γ Γ (tvar Γ) ≈ id.
+Admitted.
+
+Definition unbind : forall (Γ:env) x' σ (Hx:x' ∉ ‖Γ‖),
+  cxt ((x',σ)::Γ) → cxt Γ.
+Admitted.
+
+Lemma unbind_bind Γ x σ Hx :
+  unbind Γ x σ Hx ∘ bind Γ x σ ≈ π₁.
+Admitted.
+
+Lemma weaken_map_denote Γ Γ'
+  (VAR:varmap Γ Γ')
+  x' σ (Hx1:x' ∉ ‖Γ‖) (Hx2:x' ∉ ‖Γ'‖) :
+  varmap_denote _ _ (weaken_map Γ Γ' VAR x' σ Hx1 Hx2)
+  ≈
+  varmap_denote _ _ VAR ∘ unbind Γ' x' σ Hx2.
+Admitted.
+
+Lemma varmap_denote_proj Γ Γ' (VAR:varmap Γ Γ') x σ i :
+  〚 VAR x σ i 〛 ≈ castty i ∘ proj Γ x ∘ varmap_denote Γ Γ' VAR.
+Admitted.
+
+
+Lemma term_subst_soundness Γ τ m : forall Γ' (VAR:varmap Γ Γ'),
+  〚 term_subst Γ Γ' τ VAR m 〛 ≈ 〚m〛 ∘ varmap_denote Γ Γ' VAR.
+Proof.
+  induction m; simpl; intros.
+
+  apply varmap_denote_proj.
+
+  rewrite <- (cat_assoc PLT).
+  apply cat_respects. auto.
+  symmetry. apply plt_terminate_univ.
+
+  rewrite <- (cat_assoc PLT).
+  apply cat_respects. auto.
+  rewrite (PLT.pair_compose_commute false).
+  rewrite IHm1. rewrite IHm2. auto.
+  rewrite IHm.
+  rewrite PLT.curry_compose_commute.
+  apply PLT.curry_eq.
+  rewrite <- (cat_assoc PLT).
+  rewrite <- (cat_assoc PLT).
+  apply cat_respects; auto.
+  unfold shift_vars'.
+  unfold shift_vars.
+  rewrite varmap_extend_bind.
+  rewrite <- (cat_assoc PLT).
+  apply cat_respects; auto.
+  rewrite (PLT.pair_compose_commute false).
+  unfold PLT.pair_map.
+  apply PLT.pair_eq.
+  rewrite weaken_map_denote.
+  rewrite <- (cat_assoc PLT).
+  rewrite unbind_bind. auto.
+  simpl denote.
+  rewrite <- (cat_assoc PLT).
+  generalize (finprod.proj_bind false string string_dec ty tydom
+    Γ' (fresh_atom (‖Γ‖++‖Γ'‖++nil)) σ₁).
+  simpl. intros. 
+  etransitivity. apply cat_respects. reflexivity.
+  apply H.
+  rewrite (cat_assoc PLT).
+  match goal with 
+    [ |- castty ?H1 ∘ castty ?H2 ∘ π₂ ≈ _ ] =>
+    generalize H1 H2
   end.
+  intros.
+  etransitivity. apply cat_respects. 
+  apply (cast_compose false _ (finprod.ty false ty tydom) _ _ _ e i).
+  reflexivity.
+  etransitivity. apply cat_respects. 
+  refine (cast_dec_id false _ (finprod.ty false ty tydom) _
+    (Some σ₁) (Logic.eq_trans e i)).
+  decide equality. decide equality.
+  reflexivity.
+  auto.
+Qed.  
+
+Lemma subst_soundness Γ x σ₁ σ₂ n₁ n₂ :
+   〚 n₁ 〛 ∘ bind Γ x σ₁ ∘ 〈id, 〚 n₂ 〛〉 ≈ 〚 subst Γ σ₂ σ₁ x n₁ n₂ 〛.
+Proof.
+  unfold subst.
+  rewrite term_subst_soundness.
+  rewrite <- (cat_assoc PLT).
+  apply cat_respects; auto.
+  rewrite varmap_extend_bind.
+  rewrite varmap_var_id. auto.
+Qed.
+
+
+(**  Evaluation preserves the denotation of terms. *)
+Theorem soundness : forall Γ τ (m z:term Γ τ),
+  m ⇓ z -> 〚m〛 ≈ 〚z〛.
+Proof.
+  intros. induction H; simpl; auto.
+  rewrite IHeval1.
+  rewrite IHeval2.
+  rewrite <- IHeval3.
+  simpl.
+  rewrite PLT.curry_apply2.
+  apply subst_soundness.
+Qed.
+
+
+(**  Now we move on to the more difficult adequacy proof.
+     For this we will first need a variety of technical results
+     about the operational semantics.
+  *)
+
+Lemma eval_value Γ τ x y :
+  eval Γ τ x y -> eval Γ τ y y.
+Proof.
+  intro H. induction H.
+  apply evar.
+  apply ebool.
+  apply elam.
+  auto.
+Qed.
+
+Lemma eval_eq Γ τ x y1 y2 :
+  eval Γ τ x y1 -> eval Γ τ x y2 -> y1 = y2.
+Proof.
+  intro H. revert y2.
+  induction H.
+
+  intros. inv H. 
+  f_equal.
+  apply Eqdep_dec.UIP_dec. decide equality. decide equality.
+  intros. inv H. auto.
+  intros. inv H. auto.
+
+  intros. inv H2.
+  apply IHeval1 in H8.
+  apply IHeval2 in H9.
+  inv H8.
+  apply IHeval3; auto.
+Qed.
+
+Lemma eval_trans Γ τ x y z :
+  eval Γ τ x y -> eval Γ τ y z -> eval Γ τ x z.
+Proof.
+  intros.
+  replace z with y; auto.
+  eapply eval_eq with y; auto.
+  eapply eval_value; eauto.
+Qed.
+
+
+Lemma eval_app_congruence Γ σ₁ σ₂ : forall x x' y y' z,
+  (forall q, eval _ _ x q -> eval _ _ x' q) ->
+  (forall q, eval _ _ y q -> eval _ _ y' q) ->
+  eval Γ _ (@tapp Γ σ₁ σ₂ x y) z ->
+  eval Γ _ (@tapp Γ σ₁ σ₂ x' y') z.
+Proof.
+  intros.
+  inv H1.
+  apply H in H7.
+  apply H0 in H8.
+  eapply eapp; eauto.
+Qed.
+
+
+(**  Now we define the logical relation.  It is defined by induction
+     on the structure of types, in a standard way.
+  *)
+Fixpoint LR (τ:ty) : term nil τ -> (cxt nil → tydom τ) -> Prop :=
+  match τ as τ' return term nil τ' -> (cxt nil → tydom τ') -> Prop
+  with
+  | ty_bool => fun m h =>
+        exists b:bool, m = tbool nil b /\ 
+                h ≈ disc_elem b ∘ PLT.terminate _ _
+  | ty_arrow σ₁ σ₂ => fun m h =>
+        forall n h', 
+          LR σ₁ n h' -> eval nil σ₁ n n ->
+          exists z1 z2, 
+            eval _ _ (m•n) z1 /\
+            alpha_cong nil nil σ₂ z1 z2 /\
+            LR σ₂ z2 (apply ∘ 〈h, h'〉)
+  end.
+
+Lemma LR_equiv τ : forall m h h',
+  h ≈ h' -> LR τ m h -> LR τ m h'.
+Proof.
+  induction τ; simpl. intros.
+  destruct H0 as [b [??]]. exists b; split; auto.
+  rewrite <- H; auto.
+  simpl; intros.
+  destruct (H0 n h'0 H1 H2) as [z1 [z2 [?[??]]]].
+  exists z1; exists z2; split; auto.split; auto.
+  revert H5. apply IHτ2.
+  apply cat_respects; auto.
+  apply PLT.pair_eq; auto.
+Qed.
+
+(**  The fundamental lemma states that every term stands in the logical relation
+     with its denotation when applied to related substitutions.
+  *)
+Lemma fundamental_lemma : forall Γ τ (m:term Γ τ) 
+  (VAR:varmap Γ nil) (VARh : cxt nil → cxt Γ),
+  (forall a σ H, VAR a σ H ↓ /\
+       LR σ (VAR a σ H) (castty H ∘ proj Γ a ∘ VARh)) ->
+  exists z1 z2,
+    eval nil τ (term_subst Γ nil τ VAR m) z1 /\
+    alpha_cong nil nil τ z1 z2 /\
+    LR τ z2 (〚m〛 ∘ VARh ).
+Proof.
+  induction m; simpl; intros.
+
+  (* var case *)  
+  simpl. exists (VAR x σ i). exists (VAR x σ i). 
+  destruct (H x σ i); intuition.
+  apply alpha_eq_refl.
+  
+  (* bool case *)
+  exists (tbool nil n). 
+  exists (tbool nil n). 
+  split. apply ebool.
+  split. apply acong_bool.
+  exists n. split; auto.
+  rewrite <- (cat_assoc PLT). apply cat_respects; auto.
+  apply plt_terminate_univ.
+
+  (* application case *)  
+  destruct (IHm1 VAR VARh H) as [z1 [z1' [?[??]]]].
+  destruct (IHm2 VAR VARh H) as [z2 [z2' [?[??]]]].
+  simpl in H1.
+  destruct (H2 z2' (〚 m2 〛 ∘ VARh)) as [z3 [z3' [?[??]]]]; auto.
+admit.
+  exists z3. exists z3'.
+  split.
+  inv H6.
+  eapply eapp.
+  apply eval_trans with z1; auto. eauto. eauto.
+  replace z2 with n₂; auto.
+  apply eval_eq with z2; auto.
+  eapply eval_value; eauto.
+  revert H5.
+  apply LR_equiv.
+  rewrite <- (cat_assoc PLT).
+  apply cat_respects. auto.
+  symmetry. apply PLT.pair_compose_commute.
+
+  (* lambda case *)
+  econstructor. split. apply elam.
+  intros.
+  set (VAR' := extend_map Γ nil VAR x σ₁ n).
+  set (VARh' := bind Γ x σ₁ ∘ 〈 VARh, h' 〉). 
+  destruct (IHm VAR' VARh') as [z [??]].
+  simpl; intros.
+  split.
+  subst VAR' VARh'. unfold extend_map.
+  hnf in H2. simpl in *.
+  destruct (string_dec a x). inv H2.
+  replace H2 with (Logic.eq_refl (Some σ)). simpl.
+  unfold eq_rect_r. simpl. auto.
+  apply Eqdep_dec.UIP_dec. decide equality. decide equality.
+  apply H.
+  subst VAR' VARh'. unfold extend_map.
+  hnf in H2. simpl in *. unfold eq_rect_r. simpl.
+  unfold f_equal. unfold eq_sym. simpl.
+  revert H2.
+
+  generalize (finprod.proj_bind_neq false string string_dec ty tydom Γ x σ₁ a).
+  generalize (finprod.proj_bind false string string_dec ty tydom Γ a σ₁).
+  generalize (proj ((x,σ₁)::Γ) a).
+  unfold finprod.ty. simpl.
+  unfold finprod.lookup_neq. simpl.
+  destruct (string_dec a x). simpl; intros.
+admit.
+  intros.
+  destruct (H a σ H4). revert H6.
+  apply LR_equiv.
+  rewrite cast_refl in H3.
+  rewrite (cat_ident2 PLT) in H3.
+  rewrite <- (cat_assoc PLT).
+  rewrite <- (cat_assoc PLT).
+  rewrite (cat_assoc PLT _ _ _ _ h).
+  rewrite H3; auto.
+  rewrite <- (cat_assoc PLT).
+  rewrite PLT.pair_commute1.
+  auto.
+  exists z.
+  split.
+  eapply eapp.
+  apply elam. eauto.
+  unfold subst.
+admit. (* ?? *)
+
+  revert H3. apply LR_equiv.
+  rewrite PLT.curry_apply3.
+  unfold VARh'.
+  rewrite (cat_assoc PLT). auto.
+Qed.
+
+(**  A simpified form of the fundamental lemma that follows
+     from the inductively-strong one above.
+  *)
+Lemma fundamental_lemma' : forall τ (m:term nil τ),
+  exists z, eval nil τ m z /\ LR τ z 〚 m 〛.
+Proof.
+  intros.
+  destruct (fundamental_lemma nil τ m (tvar nil) id) as [z [??]].
+  intros. hnf in H. simpl in H. discriminate.
+  exists z. split.
+admit.
+  revert H0. apply LR_equiv.
+  apply cat_ident1.
+Qed.
+
+
+(**  Now we define contextual equivalance.  Contexts here are
+     given in "inside-out" form, which makes the induction in the
+     adequacy proof significantly easier.
+  *)
+
+Inductive context τ : env -> ty -> Type :=
+  | cxt_top : context τ nil τ
+  | cxt_appl : forall Γ σ₁ σ₂,
+                    term Γ σ₁ ->
+                    context τ Γ σ₂ ->
+                    context τ Γ (σ₁ ⇒ σ₂)
+  | cxt_appr : forall Γ σ₁ σ₂,
+                    term Γ (σ₁ ⇒ σ₂) ->
+                    context τ Γ σ₂ ->
+                    context τ Γ σ₁
+  | cxt_lam : forall Γ (x:atom) σ₁ σ₂,
+                    context τ Γ (σ₁ ⇒ σ₂) ->
+                    context τ ((x,σ₁)::Γ) σ₂.
+
+Fixpoint plug τ Γ σ (C:context τ Γ σ) : term Γ σ -> term nil τ :=
+  match C in context _ Γ' σ' return term Γ' σ' -> term nil τ with
+  | cxt_top => fun x => x
+  | cxt_appl Γ σ₁ σ₂ t C' => fun x => plug τ _ _ C' (tapp x t)
+  | cxt_appr Γ σ₁ σ₂ t C' => fun x => plug τ _ _ C' (tapp t x)
+  | cxt_lam  Γ a σ₁ σ₂ C' => fun x => plug τ _ _ C' (tlam Γ a σ₁ σ₂ x)
+  end.
+
+Definition cxt_eq τ Γ σ (m n:term Γ σ):=
+  forall (C:context τ Γ σ) (z:term nil τ),
+    eval nil τ (plug τ Γ σ C m) z <-> eval nil τ (plug τ Γ σ C n) z.
+
+Lemma terminate_le_cancel (hf:bool) (A B:PLT.PLT hf) (f g:1 → B) (a:A) :
+  f ∘ PLT.terminate hf A ≤ g ∘ PLT.terminate hf A ->
+  f ≤ g.
+Proof.
+  repeat intro.
+  destruct a0. destruct c.
+  assert ((a,c0) ∈ PLT.hom_rel (f ∘ PLT.terminate hf A)).
+  apply PLT.compose_hom_rel. exists tt. split; auto.
+  apply eprod_elem. split; apply eff_complete.
+  apply H in H1.
+  apply PLT.compose_hom_rel in H1.
+  destruct H1 as [[] [??]]. auto.
+Qed.
+
+Lemma terminate_cancel (hf:bool) (A B:PLT.PLT hf) (f g:1 → B) (a:A) :
+  f ∘ PLT.terminate hf A ≈ g ∘ PLT.terminate hf A ->
+  f ≈ g.
+Proof.
+  intros. destruct H; split; eapply terminate_le_cancel; eauto.
+Qed.
+
+(**  Adequacy means that terms with equivalant denotations
+     are contextually equivalant in any boolean context.
+  *)
+Theorem adequacy : forall Γ τ (m n:term Γ τ),
+  〚m〛 ≈ 〚n〛 -> cxt_eq ty_bool Γ τ m n.
+Proof.
+  intros. intro.
+  revert n m H.
+  induction C.
+
+  simpl; intros.
+  destruct (fundamental_lemma' _ m) as [zm [??]]. simpl in *.
+  destruct (fundamental_lemma' _ n) as [zn [??]]. simpl in *.
+  destruct H1 as [bm [??]].
+  destruct H3 as [bn [??]].
+  subst zm zn.
+  rewrite H in H4.
+  rewrite H4 in H5.
+  assert (bm = bn).
+  apply (terminate_cancel false (cxt nil) _ _ _ (fun i => tt)) in H5.
+  apply disc_elem_inj in H5. auto.
+  subst bn.
+  split; intro.
+  assert (z = (tbool nil bm)).
+  eapply eval_eq; eauto.
+  subst z. auto.
+  assert (z = (tbool nil bm)).
+  eapply eval_eq; eauto.
+  subst z. auto.
+
+  simpl. intros.
+  apply IHC. simpl.
+  apply cat_respects; auto.
+  apply PLT.pair_eq; auto.
+
+  simpl; intros.
+  apply IHC. simpl.
+  apply cat_respects; auto.
+  apply PLT.pair_eq; auto.
+
+  simpl; intros.
+  apply IHC. simpl.
+  apply PLT.curry_eq.
+  apply cat_respects; auto.
+Qed.
+
+(**  As a corollary of the fundamental lemma, we learn that
+     the calculus is strongly normalizing.
+  *)
+Corollary normalizing : forall τ (m:term nil τ), exists z, eval nil τ m z.
+Proof.
+  intros.
+  generalize (fundamental_lemma' τ m).
+  simpl. intros [z [??]]. exists z; auto.
+Qed.
+
+(** These should print "Closed under the global context", meaning these
+    theorems hold without the use of any axioms.
+  *)
+Print Assumptions adequacy.
+Print Assumptions normalizing.
